Rename operations and lemmas

SystemF/Subst/Tm.lean
@@ -4,87 +4,86 @@ namespace SystemF
 
 open Notation
 
-
 /-- Open `t` with `u` at index `k`. -/
-def openTm (k : ℕ) (u t : Tm) : Tm :=
+def Tm.open (t : Tm) (k : ℕ) (u : Tm) : Tm :=
   match t with
   | .bvar x => if x == k then u else .bvar x
-  | .tLam t => .tLam (openTm k u t)
-  | .lam ty t => .lam ty (openTm (k + 1) u t)
-  | .app t₁ t₂ => .app (openTm k u t₁) (openTm k u t₂)
-  | .tApp t T => .tApp (openTm k u t) T
+  | .tLam t => .tLam (t.open k u)
+  | .lam ty t => .lam ty (t.open (k + 1) u)
+  | .app t₁ t₂ => .app (t₁.open k u) (t₂.open k u)
+  | .tApp t T => .tApp (t.open k u) T
   | .fvar x => .fvar x
 
 instance : Open Tm Tm where
-  «open» := openTm
+  «open» k u t := t.open k u
 
 @[simp, grind =]
-lemma openTm_bvar {k : ℕ} {u : Tm} {x : ℕ} :
+lemma Tm.open_bvar {k : ℕ} {u : Tm} {x : ℕ} :
   (#v x)⟪k, u⟫ = if x == k then u else #v x := rfl
 
 @[simp, grind =]
-lemma openTm_fvar {k : ℕ} {u : Tm} {X : Name} :
+lemma Tm.open_fvar {k : ℕ} {u : Tm} {X : Name} :
   ($v X)⟪k, u⟫ = $v X := rfl
 
 @[simp, grind =]
-lemma openTm_lam {k : ℕ} {u : Tm} {T : Ty} {t : Tm} :
+lemma Tm.open_lam {k : ℕ} {u : Tm} {T : Ty} {t : Tm} :
   (ƛ T => t)⟪k, u⟫ = (ƛ T => t⟪k + 1, u⟫) := rfl
 
 @[simp, grind =]
-lemma openTm_app {k : ℕ} {u : Tm} {t₁ t₂ : Tm} :
+lemma Tm.open_app {k : ℕ} {u : Tm} {t₁ t₂ : Tm} :
   (t₁ ◦ t₂)⟪k, u⟫ = (t₁⟪k, u⟫ ◦ t₂⟪k, u⟫) := rfl
 
 @[simp, grind =]
-lemma openTm_tLam {k : ℕ} {u : Tm} {t : Tm} :
+lemma Tm.open_tLam {k : ℕ} {u : Tm} {t : Tm} :
   (Λ' t)⟪k, u⟫ = Λ' (t⟪k, u⟫) := rfl
 
 @[simp, grind =]
-lemma openTm_tApp {k : ℕ} {u : Tm} {t : Tm} {T : Ty} :
+lemma Tm.open_tApp {k : ℕ} {u : Tm} {t : Tm} {T : Ty} :
   (t ⦃T⦄)⟪k, u⟫ = (t⟪k, u⟫⦃T⦄) := rfl
 
-def substTm (X : Name) (u t : Tm) : Tm :=
+def Tm.subst (t : Tm) (X : Name) (u : Tm) : Tm :=
   match t with
   | .bvar idx => .bvar idx
   | .fvar name => if name == X then u else .fvar name
-  | .app t₁ t₂ => .app (substTm X u t₁) (substTm X u t₂)
-  | .lam T t => .lam T (substTm X u t)
-  | .tLam t => .tLam (substTm X u t)
-  | .tApp t T => .tApp (substTm X u t) T
+  | .app t₁ t₂ => .app (t₁.subst X u) (t₂.subst X u)
+  | .lam T t => .lam T (t.subst X u)
+  | .tLam t => .tLam (t.subst X u)
+  | .tApp t T => .tApp (t.subst X u) T
 
 instance : Subst Tm Tm where
-  subst := substTm
+  subst X u t := t.subst X u
 
 @[simp, grind =]
-lemma substTm_bvar {X : Name} {u : Tm} {idx : ℕ} :
+lemma Tm.subst_bvar {X : Name} {u : Tm} {idx : ℕ} :
   (Tm.bvar idx)[X ↦ u] = Tm.bvar idx := rfl
 
 @[simp, grind =]
-lemma substTm_fvar {X : Name} {u : Tm} {name : Name} :
+lemma Tm.subst_fvar {X : Name} {u : Tm} {name : Name} :
   (Tm.fvar name)[X ↦ u] = if name == X then u else Tm.fvar name := rfl
 
 @[simp, grind =]
-lemma substTm_app {X : Name} {u : Tm} {t₁ t₂ : Tm} :
+lemma Tm.subst_app {X : Name} {u : Tm} {t₁ t₂ : Tm} :
   (Tm.app t₁ t₂)[X ↦ u] = Tm.app (t₁[X ↦ u]) (t₂[X ↦ u]) := rfl
 
 @[simp, grind =]
-lemma substTm_lam {X : Name} {u : Tm} {T : Ty} {t : Tm} :
+lemma Tm.subst_lam {X : Name} {u : Tm} {T : Ty} {t : Tm} :
   (Tm.lam T t)[X ↦ u] = Tm.lam T (t[X ↦ u]) := rfl
 
 @[simp, grind =]
-lemma substTm_tLam {X : Name} {u : Tm} {t : Tm} :
+lemma Tm.subst_tLam {X : Name} {u : Tm} {t : Tm} :
   (Tm.tLam t)[X ↦ u] = Tm.tLam (t[X ↦ u]) := rfl
 
 @[simp, grind =]
-lemma substTm_tApp {X : Name} {u : Tm} {t : Tm} {T : Ty} :
+lemma Tm.subst_tApp {X : Name} {u : Tm} {t : Tm} {T : Ty} :
   (Tm.tApp t T)[X ↦ u] = Tm.tApp (t[X ↦ u]) T := rfl
 
 @[simp]
-lemma substTm_fresh {t : Tm} {X : Name} {u : Tm} (h : X ∉ t.fv) :
+lemma Tm.subst_fresh {t : Tm} {X : Name} {u : Tm} (h : X ∉ t.fv) :
     t[X ↦ u] = t := by
   induction t <;> grind
 
 @[grind =]
-theorem substTm_openTm_var {t u : Tm} {x : Name} {k : ℕ} (h : x ∉ t.fv) :
+theorem Tm.subst_open_var {t u : Tm} {x : Name} {k : ℕ} (h : x ∉ t.fv) :
     (t⟪k, $v x⟫)[x ↦ u] = t⟪k, u⟫ := by
   induction t generalizing k <;> grind
 
