SystemF/Subst/TyTm.lean
@@ -8,96 +8,98 @@ open Notation
 /-- Open `t` with `U` at index `k`.
   Only handles type variables abstracted by `tLam`.
 -/
-def openTmTy (k : ℕ) (U : Ty) (t : Tm) : Tm :=
+def Tm.openTy (t : Tm) (k : ℕ) (U : Ty) : Tm :=
   match t with
   | .bvar x => .bvar x
-  | .app t₁ t₂ => .app (openTmTy k U t₁) (openTmTy k U t₂)
-  | .lam T' t => .lam (openTy k U T') (openTmTy k U t)
-  | .tLam t => .tLam (openTmTy (k + 1) U t)
-  | .tApp t T' => .tApp (openTmTy k U t) (openTy k U T')
+  | .app t₁ t₂ => .app (t₁.openTy k U) (t₂.openTy k U)
+  | .lam T' t => .lam (T'.open k U) (t.openTy k U)
+  | .tLam t => .tLam (t.openTy (k + 1) U)
+  | .tApp t T' => .tApp (t.openTy k U) (T'.open k U)
   | .fvar x => .fvar x
 
 instance : Open Ty Tm where
-  «open» := openTmTy
+  «open» k U t := t.openTy k U
 
 @[simp, grind =]
-lemma openTmTy_bvar {k : ℕ} {U : Ty} {x : ℕ} :
+lemma Tm.openTy_bvar {k : ℕ} {U : Ty} {x : ℕ} :
   (#v x)⟪k, U⟫ = #v x := rfl
 
 @[simp, grind =]
-lemma openTmTy_fvar {k : ℕ} {U : Ty} {X : Name} :
+lemma Tm.openTy_fvar {k : ℕ} {U : Ty} {X : Name} :
   ($v X)⟪k, U⟫ = $v X := rfl
 
 @[simp, grind =]
-lemma openTmTy_lam {k : ℕ} {U : Ty} {T : Ty} {t : Tm} :
+lemma Tm.openTy_lam {k : ℕ} {U : Ty} {T : Ty} {t : Tm} :
   (ƛ T => t)⟪k, U⟫ = (ƛ (T⟪k, U⟫) => t⟪k, U⟫) := rfl
 
 @[simp, grind =]
-lemma openTmTy_app {k : ℕ} {U : Ty} {t₁ t₂ : Tm} :
+lemma Tm.openTy_app {k : ℕ} {U : Ty} {t₁ t₂ : Tm} :
   (t₁ ◦ t₂)⟪k, U⟫ = (t₁⟪k, U⟫ ◦ t₂⟪k, U⟫) := rfl
 
 @[simp, grind =]
-lemma openTmTy_tLam {k : ℕ} {U : Ty} {t : Tm} :
+lemma Tm.openTy_tLam {k : ℕ} {U : Ty} {t : Tm} :
   (Λ' t)⟪k, U⟫ = Λ' (t⟪k + 1, U⟫) := rfl
 
 @[simp, grind =]
-lemma openTmTy_tApp {k : ℕ} {U : Ty} {t : Tm} {T : Ty} :
+lemma Tm.openTy_tApp {k : ℕ} {U : Ty} {t : Tm} {T : Ty} :
   (t ⦃T⦄)⟪k, U⟫ = (t⟪k, U⟫ ⦃T⟪k, U⟫⦄) := rfl
 
 /-- Substitute free type variable `X` with `U` in term `t`. -/
-def substTmTy (X : Name) (U : Ty) (t : Tm) : Tm :=
+def Tm.substTy (t : Tm) (X : Name) (U : Ty) : Tm :=
   match t with
   | .bvar idx => .bvar idx
   | .fvar name => .fvar name
-  | .app t₁ t₂ => .app (substTmTy X U t₁) (substTmTy X U t₂)
-  | .lam T t => .lam (substTy X U T) (substTmTy X U t)
-  | .tLam t => .tLam (substTmTy X U t)
-  | .tApp t T => .tApp (substTmTy X U t) (substTy X U T)
+  | .app t₁ t₂ => .app (t₁.substTy X U) (t₂.substTy X U)
+  | .lam T t => .lam (T.subst X U) (t.substTy X U)
+  | .tLam t => .tLam (t.substTy X U)
+  | .tApp t T => .tApp (t.substTy X U) (T.subst X U)
 
 instance : Subst Ty Tm where
-  subst := substTmTy
+  subst X U t := t.substTy X U
 
 @[simp, grind =]
-lemma substTmTy_bvar {X : Name} {U : Ty} {idx : ℕ} :
+lemma Tm.substTy_bvar {X : Name} {U : Ty} {idx : ℕ} :
   (Tm.bvar idx)[X ↦ U] = Tm.bvar idx := rfl
 
 @[simp, grind =]
-lemma substTmTy_fvar {X : Name} {U : Ty} {name : Name} :
+lemma Tm.substTy_fvar {X : Name} {U : Ty} {name : Name} :
   (Tm.fvar name)[X ↦ U] = Tm.fvar name := rfl
 
 @[simp, grind =]
-lemma substTmTy_app {X : Name} {U : Ty} {t₁ t₂ : Tm} :
+lemma Tm.substTy_app {X : Name} {U : Ty} {t₁ t₂ : Tm} :
   (Tm.app t₁ t₂)[X ↦ U] = Tm.app (t₁[X ↦ U]) (t₂[X ↦ U]) := rfl
 
 @[simp, grind =]
-lemma substTmTy_lam {X : Name} {U : Ty} {T : Ty} {t : Tm} :
+lemma Tm.substTy_lam {X : Name} {U : Ty} {T : Ty} {t : Tm} :
   (Tm.lam T t)[X ↦ U] = Tm.lam (T[X ↦ U]) (t[X ↦ U]) := rfl
 
 @[simp, grind =]
-lemma substTmTy_tLam {X : Name} {U : Ty} {t : Tm} :
+lemma Tm.substTy_tLam {X : Name} {U : Ty} {t : Tm} :
   (Tm.tLam t)[X ↦ U] = Tm.tLam (t[X ↦ U]) := rfl
 
 @[simp, grind =]
-lemma substTmTy_tApp {X : Name} {U : Ty} {t : Tm} {T : Ty} :
+lemma Tm.substTy_tApp {X : Name} {U : Ty} {t : Tm} {T : Ty} :
   (Tm.tApp t T)[X ↦ U] = Tm.tApp (t[X ↦ U]) (T[X ↦ U]) := rfl
 
 @[simp]
-lemma substTmTy_fresh {t : Tm} {X : Name} {U : Ty} (h : X ∉ t.fvTy) :
+lemma Tm.substTy_fresh {t : Tm} {X : Name} {U : Ty} (h : X ∉ t.fvTy) :
     t[X ↦ U] = t := by
-  induction t <;> grind [substTy_fresh]
+  induction t <;> grind [Ty.subst_fresh]
 
-theorem openTm_substTmTy_comm {t u : Tm} {X : Name} {U : Ty} {k : ℕ} :
-    (t[X ↦ U])⟪k, u[X ↦ U]⟫ = (t⟪k, u⟫)[X ↦ U]:= by
+theorem Tm.open_substTy_comm {t u : Tm} {X : Name} {U : Ty} {k : ℕ} :
+    (t[X ↦ U])⟪k, u[X ↦ U]⟫ = (t⟪k, u⟫)[X ↦ U] := by
   induction t generalizing k <;> grind
 
-theorem openTm_substTmTy_comm_fresh {t u : Tm} {X : Name} {U : Ty} {k : ℕ} (h : X ∉ u.fvTy) :
-     (t[X ↦ U])⟪k, u⟫ = (t⟪k, u⟫)[X ↦ U] := by
-  rw [←substTmTy_fresh h]
-  rw [openTm_substTmTy_comm]
-  rw [substTmTy_fresh h]
+theorem Tm.open_substTy_comm_fresh {t u : Tm} {X : Name} {U : Ty} {k : ℕ}
+    (h : X ∉ u.fvTy) :
+    (t[X ↦ U])⟪k, u⟫ = (t⟪k, u⟫)[X ↦ U] := by
+  rw [←Tm.substTy_fresh h]
+  rw [Tm.open_substTy_comm]
+  rw [Tm.substTy_fresh h]
 
 @[grind =]
-theorem substTmTy_openTmTy_var {t : Tm} {U : Ty} {X : Name} {k : ℕ} (h : X ∉ t.fvTy) :
+theorem Tm.substTy_openTy_var {t : Tm} {U : Ty} {X : Name} {k : ℕ}
+    (h : X ∉ t.fvTy) :
     (t⟪k, $T X⟫)[X ↦ U] = t⟪k, U⟫ := by
   induction t generalizing k <;> grind
 
