SystemF/Lc/Norm.lean
@@ -6,15 +6,15 @@ namespace SystemF
 open Notation
 
 @[ln_norm_simps]
-theorem substTy_refold (X : Name) (U T : Ty) :
-    substTy X U T = T[X ↦ U] := rfl
+theorem Ty.subst_refold (X : Name) (U T : Ty) :
+    T.subst X U = T[X ↦ U] := rfl
 
 @[ln_norm_simps]
-theorem substTm_refold (x : Name) (u t : Tm) :
-    substTm x u t = t[x ↦ u] := rfl
+theorem Tm.subst_refold (x : Name) (u t : Tm) :
+    t.subst x u = t[x ↦ u] := rfl
 
 @[ln_norm_simps]
-theorem substTmTy_refold (X : Name) (U : Ty) (t : Tm) :
-    substTmTy X U t = t[X ↦ U] := rfl
+theorem Tm.substTy_refold (X : Name) (U : Ty) (t : Tm) :
+    t.substTy X U = t[X ↦ U] := rfl
 
 end SystemF
