SystemF/Lc/Tm.lean
@@ -18,60 +18,62 @@ example : ¬ LcTm (ƛ ($T "A") => #v 1) := by
   intro h
   cases h with
   | lam L T t h₁ h₂ =>
-    simp only [openTm_bvar, Nat.reduceBEq, Bool.false_eq_true, ↓reduceIte] at h₂
+    simp only [Tm.open_bvar, Nat.reduceBEq, Bool.false_eq_true, ↓reduceIte] at h₂
     pick_fresh x
     specialize h₂ x hx
     cases h₂
 
-theorem openTm_neq_id {k j : ℕ} {t u v : Tm} (hNeq : k ≠ j) (h : t⟪j, v⟫⟪k, u⟫ = t⟪j, v⟫) :
+theorem Tm.open_neq_id {k j : ℕ} {t u v : Tm} (hNeq : k ≠ j) (h : t⟪j, v⟫⟪k, u⟫ = t⟪j, v⟫) :
     t⟪k, u⟫ = t := by
-  induction t generalizing k j <;> simp at * <;> grind
+  induction t generalizing k j <;> grind
 
-theorem openTm_eq_id {k j : ℕ} {t v : Tm} {U : Ty} (h : t⟪j, U⟫⟪k, v⟫ = t⟪j, U⟫) :
+
+theorem Tm.open_eq_id {k j : ℕ} {t v : Tm} {U : Ty} (h : t⟪j, U⟫⟪k, v⟫ = t⟪j, U⟫) :
     t⟪k, v⟫ = t := by
-  induction t generalizing k j <;> simp at * <;> grind
+  induction t generalizing k j <;> grind
 
 @[simp]
-theorem openTm_lcTm_id {u : Tm} (h : LcTm u) (k : ℕ) (v : Tm) :
+theorem Tm.open_lc_id {u : Tm} (h : LcTm u) (k : ℕ) (v : Tm) :
     u⟪k, v⟫ = u := by
   induction h generalizing k v with
   | fvar x => simp
   | app t₁ t₂ _ _ _ _ => grind
   | lam L T t _ _ ih =>
-    simp only [openTm_lam, Tm.lam.injEq, true_and]
+    simp only [open_lam, lam.injEq, true_and]
     pick_fresh x
     have := ih x (by grind) (k + 1) v
-    have := @openTm_neq_id (k + 1) 0 t v ($vx) (by grind) (by assumption)
+    have := @Tm.open_neq_id (k + 1) 0 t v ($vx) (by grind) (by assumption)
     rw [this]
   | tApp t T _ _ _ => grind
   | tLam L t _ ih =>
-    simp only [openTm_tLam, Tm.tLam.injEq]
+    simp only [open_tLam, tLam.injEq]
     pick_fresh X
     specialize ih X (by grind) k v
-    have := openTm_eq_id ih
+    have := open_eq_id ih
     rw [this]
 
-theorem openTm_substTm_comm {t u v : Tm} {X : Name} {k : ℕ} (hu : LcTm u) :
+
+theorem Tm.open_subst_comm {t u v : Tm} {X : Name} {k : ℕ} (hu : LcTm u) :
     (t[X ↦ u])⟪k, v[X ↦ u]⟫ = (t⟪k, v⟫)[X ↦ u]:= by
-  induction t generalizing k <;> simp at * <;> grind [openTm_lcTm_id]
+  induction t generalizing k <;> simp at * <;> grind [open_lc_id]
 
 @[ln_norm_simps]
-theorem openTm_substTm_comm_of_neq {t u : Tm} {x y : Name} {k : ℕ}
+theorem Tm.open_subst_comm_of_neq {t u : Tm} {x y : Name} {k : ℕ}
     (hNeq : y ≠ x) (hu : LcTm u) :
     (t[x ↦ u])⟪k, $vy⟫ = (t⟪k, $vy⟫)[x ↦ u] := by
-  rw [←openTm_substTm_comm hu]
+  rw [←open_subst_comm hu]
   simp [hNeq]
 
-theorem psubst_openTm_comm' {k} {t v : Tm} {x : Name} {γ : TmSubst} {δ : TySubst}
+theorem Tm.psubst_open_comm_update {k} {t v : Tm} {x : Name} {γ : TmSubst} {δ : TySubst}
     (hx : x ∉ t.fv)
     (hγ : ∀ y, LcTm (γ y)) :
     (t.psubst γ δ)⟪k, v⟫ = (t⟪k, $v x⟫).psubst (Function.update γ x v) δ := by
-  induction t generalizing x k with grind [Tm.psubst, openTm_lcTm_id]
+  induction t generalizing x k with grind [psubst, open_lc_id]
 
-theorem psubst_openTm_comm {k} {t : Tm} {x : Name} {γ : TmSubst} {δ : TySubst}
+theorem Tm.psubst_open_comm {k} {t : Tm} {x : Name} {γ : TmSubst} {δ : TySubst}
     (hx : x ∉ t.fv)
     (hγ : ∀ y, LcTm (γ y)) :
     (t.psubst γ δ)⟪k, $v x⟫ = (t⟪k, $v x⟫).psubst (Function.update γ x ($v x)) δ := by
-  apply psubst_openTm_comm' hx hγ
+  apply psubst_open_comm_update hx hγ
 
 end SystemF
