SystemF/Lc/Ty.lean
@@ -11,30 +11,32 @@ example : LcTy (∀' (#T 0 ⇒ #T 0)) := by
   apply_cofinite
   grind [LcTy.fvar, LcTy.arr]
 
-theorem openTy_neq_id {k j : ℕ} {T U V : Ty} (hNeq : k ≠ j) (h : T⟪j, V⟫⟪k, U⟫ = T⟪j, V⟫) :
+theorem Ty.open_neq_id {k j : ℕ} {T U V : Ty} (hNeq : k ≠ j) (h : T⟪j, V⟫⟪k, U⟫ = T⟪j, V⟫) :
     T⟪k, U⟫ = T := by
   induction T generalizing k j <;> grind
 
 @[simp]
-theorem openTy_lcTy_id {U : Ty} (h : LcTy U) (k : ℕ) (V : Ty) :
+theorem Ty.open_lc_id {U : Ty} (h : LcTy U) (k : ℕ) (V : Ty) :
     U⟪k, V⟫ = U := by
   induction h generalizing k V with
   | fvar x => grind [LcTy.fvar]
   | arr T₁ T₂ _ _ ih₁ ih₂ => grind [LcTy.arr]
   | all L T _ ih =>
-    simp only [openTy_all, Ty.all.injEq]
+    simp only [open_all, all.injEq]
     pick_fresh X
-    grind [openTy_neq_id]
+    grind [open_neq_id]
+
 
 /-- Substitution commutes with opening on types -/
 @[ln_norm_simps]
-theorem openTy_substTy_comm {k} {X Y : Name} {T U : Ty} (hNeq : X ≠ Y) (hU : LcTy U) :
+theorem Ty.open_subst_comm {k} {X Y : Name} {T U : Ty} (hNeq : X ≠ Y) (hU : LcTy U) :
     (T[X ↦ U])⟪k, ($T Y)⟫ = (T⟪k, $T Y⟫)[X ↦ U] := by
   induction T generalizing k <;> aesop
 
+
 /-- Substitution preserves locally closedness of types -/
 @[aesop safe apply (rule_sets := [LcRules])]
-theorem substTy_lcTy {T U : Ty} {X : Name} (hT : LcTy T) (hU : LcTy U) : LcTy (T[X ↦ U]) := by
+theorem Ty.subst_lc {T U : Ty} {X : Name} (hT : LcTy T) (hU : LcTy U) : LcTy (T[X ↦ U]) := by
   induction hT with
   | fvar x => grind [LcTy.fvar]
   | arr T₁ T₂ _ _ ih₁ ih₂ => grind [LcTy.arr]
@@ -44,34 +46,37 @@ theorem substTy_lcTy {T U : Ty} {X : Name} (hT : LcTy T) (hU : LcTy U) : LcTy (T
     intro X hX
     ln_norm
 
-theorem substTy_dist_openTy {T U V : Ty} {X : Name} {k : ℕ} (hU : LcTy U) :
+
+theorem Ty.subst_dist_open {T U V : Ty} {X : Name} {k : ℕ} (hU : LcTy U) :
     (T⟪k, V⟫)[X ↦ U] = (T[X ↦ U])⟪k, V[X ↦ U]⟫ := by
-  induction T generalizing k <;> grind [openTy_lcTy_id]
+  induction T generalizing k <;> grind [open_lc_id]
+
 
 /-- If `∀' T` is locally closed (meaning `T` is not closed) and `U` is locally closed,
   then opening `T` with `U` yields a locally closed type.
 -/
 @[grind ., aesop unsafe 50% apply (rule_sets := [LcRules])]
-theorem openTy_lcTy {T U : Ty} (hT : LcTy (∀' T)) (hU : LcTy U) : LcTy (T⟪U⟫) := by
+theorem Ty.open_lc {T U : Ty} (hT : LcTy (∀' T)) (hU : LcTy U) : LcTy (T⟪U⟫) := by
   cases hT with
   | all L T h =>
     pick_fresh X
     specialize h X (by grind)
-    have := substTy_lcTy (X := X) h hU
-    rw [←substTy_openTy_var (X := X) (by grind)]
+    have := subst_lc (X := X) h hU
+    rw [←subst_open_var (X := X) (by grind)]
     apply this
 
-theorem psubst_openTy_comm' {k} {T U : Ty} {X : Name} {δ : Name → Ty}
+
+theorem Ty.psubst_open_comm_update {k} {T U : Ty} {X : Name} {δ : Name → Ty}
     (hX : X ∉ T.fv)
     (hδ : ∀ Y, LcTy (δ Y)) :
     (T.psubst δ)⟪k, U⟫ = (T⟪k, $TX⟫).psubst (Function.update δ X U) := by
-  induction T generalizing X k with grind [Ty.psubst, openTy_lcTy_id]
+  induction T generalizing X k with grind [psubst, open_lc_id]
 
-theorem psubst_openTy_comm {k} {T : Ty} {X : Name} {δ : TySubst}
+theorem Ty.psubst_open_comm {k} {T : Ty} {X : Name} {δ : TySubst}
     (hX : X ∉ T.fv)
     (hδ : ∀ Y, LcTy (δ Y)) :
     (T.psubst δ)⟪k, $TX⟫ = (T⟪k, $TX⟫).psubst (Function.update δ X ($T X)) := by
-  apply psubst_openTy_comm' hX hδ
+  apply psubst_open_comm_update hX hδ
 
 @[aesop safe apply (rule_sets := [LcRules])]
 lemma psubst_lcTy {T : Ty} (hLc : LcTy T) {δ : TySubst}
@@ -82,7 +87,7 @@ lemma psubst_lcTy {T : Ty} (hLc : LcTy T) {δ : TySubst}
     constructor <;> grind
   | all L T _ ih =>
     apply_cofinite
-    grind [psubst_openTy_comm, LcTy.fvar]
+    grind [Ty.psubst_open_comm, LcTy.fvar]
 
 def Ty.LcAt (T : Ty) (k : ℕ) : Prop :=
   match T with
@@ -91,17 +96,16 @@ def Ty.LcAt (T : Ty) (k : ℕ) : Prop :=
   | .arr T₁ T₂ => T₁.LcAt k ∧ T₂.LcAt k
   | .all T => T.LcAt (k + 1)
 
-
-theorem lcAtTy_of_openTy {T : Ty} {X : Name} {k : ℕ}
+theorem Ty.lcAt_of_open {T : Ty} {X : Name} {k : ℕ}
     (h : (T⟪k, $TX⟫).LcAt k) : T.LcAt (k + 1) := by
   induction T generalizing k with grind [Ty.LcAt]
 
-theorem lcAt_zero_of_lcTy {T : Ty} (h : LcTy T) : T.LcAt 0 := by
+theorem Ty.lcAt_zero_of_lc {T : Ty} (h : LcTy T) : T.LcAt 0 := by
   induction h with
-  | fvar x => simp [Ty.LcAt]
-  | arr T₁ T₂ _ _ _ _ => simp [Ty.LcAt] at *; grind
+  | fvar x => simp [LcAt]
+  | arr T₁ T₂ _ _ _ _ => grind [LcAt]
   | all L T _ ih =>
     pick_fresh _
-    grind [lcAtTy_of_openTy, Ty.LcAt]
+    grind [lcAt_of_open, LcAt]
 
 end SystemF
