SystemF/Lc/TyTm.lean
@@ -4,103 +4,104 @@ namespace SystemF
 
 open Notation
 
-attribute [ln_norm_simps] openTm_substTmTy_comm_fresh
+attribute [ln_norm_simps] Tm.open_substTy_comm_fresh
 
 @[ln_norm_simps]
-theorem openTmTy_substTmTy_comm {t : Tm} {U : Ty} {X Y : Name} {k : ℕ}
+theorem Tm.openTy_substTy_comm {t : Tm} {U : Ty} {X Y : Name} {k : ℕ}
     (hNeq : X ≠ Y) (hU : LcTy U) :
     (t[X ↦ U])⟪k, ($T Y)⟫ = (t⟪k, ($T Y)⟫)[X ↦ U] := by
-  induction t generalizing k <;> grind [openTy_substTy_comm]
+  induction t generalizing k <;> grind [Ty.open_subst_comm]
 
-lemma openTmTy_substTmTy_comm' {t : Tm} {X : Name} {U V : Ty} {k : ℕ}
+lemma Tm.openTy_substTy_comm_of_lc {t : Tm} {X : Name} {U V : Ty} {k : ℕ}
     (hU : LcTy U) :
     (t[X ↦ U])⟪k, V[X ↦ U]⟫ = (t⟪k, V⟫)[X ↦ U] := by
-  induction t generalizing k <;> grind [substTy_dist_openTy]
+  induction t generalizing k <;> grind [Ty.subst_dist_open]
 
-theorem openTmTy_eq_id {k j : ℕ} {t u : Tm} {T : Ty} (h : t⟪j, u⟫⟪k, T⟫ = t⟪j, u⟫) :
+theorem Tm.openTy_eq_id {k j : ℕ} {t u : Tm} {T : Ty} (h : t⟪j, u⟫⟪k, T⟫ = t⟪j, u⟫) :
     t⟪k, T⟫ = t := by
-  induction t generalizing k j <;> simp at * <;> grind [openTy_neq_id]
+  induction t generalizing k j <;> simp at * <;> grind [Ty.open_neq_id]
 
-theorem openTmTy_neq_id {k j : ℕ} {t : Tm} {T U : Ty} (hNeq : k ≠ j) (h : t⟪j, U⟫⟪k, T⟫ = t⟪j, U⟫) :
+theorem Tm.openTy_neq_id {k j : ℕ} {t : Tm} {T U : Ty}
+    (hNeq : k ≠ j) (h : t⟪j, U⟫⟪k, T⟫ = t⟪j, U⟫) :
     t⟪k, T⟫ = t := by
-  induction t generalizing k j <;> simp at * <;> grind [openTy_neq_id]
+  induction t generalizing k j <;> simp at * <;> grind [Ty.open_neq_id]
 
 @[simp]
-theorem openTmTy_lcTm_id {u : Tm} (hu : LcTm u) (k : ℕ) (V : Ty) :
+theorem Tm.openTy_lc_id {u : Tm} (hu : LcTm u) (k : ℕ) (V : Ty) :
     u⟪k, V⟫ = u := by
   induction hu generalizing k V with
   | fvar x => simp
   | app t₁ t₂ _ _ _ _ => grind
   | lam L T t hT _ ih =>
-    simp only [openTmTy_lam, Tm.lam.injEq]
+    simp only [openTy_lam, lam.injEq]
     constructor
-    · apply openTy_lcTy_id hT
-    · pick_fresh _; grind [openTmTy_eq_id]
-  | tApp t T _ _ ih => grind [openTy_lcTy_id]
+    · aesop
+    · pick_fresh _; grind [openTy_eq_id]
+  | tApp t T _ _ ih => grind [Ty.open_lc_id]
   | tLam L _ _ ih =>
     pick_fresh _
-    grind [openTmTy_neq_id]
+    grind [openTy_neq_id]
 
 @[ln_norm_simps]
-theorem openTmTy_substTm_comm {t u : Tm} {x : Name} {V : Ty} {k : ℕ} (hu : LcTm u) :
+theorem Tm.openTy_subst_comm {t u : Tm} {x : Name} {V : Ty} {k : ℕ} (hu : LcTm u) :
     (t⟪k, V⟫)[x ↦ u] = (t[x ↦ u])⟪k, V⟫ := by
-  induction t generalizing k <;> grind [openTmTy_lcTm_id]
+  induction t generalizing k <;> grind [openTy_lc_id]
 
 @[aesop safe apply (rule_sets := [LcRules])]
-theorem substTm_lcTm {t u : Tm} {x : Name} (ht : LcTm t) (hu : LcTm u) : LcTm (t[x ↦ u]) := by
+theorem Tm.subst_lc {t u : Tm} {x : Name} (ht : LcTm t) (hu : LcTm u) : LcTm (t[x ↦ u]) := by
   induction ht generalizing x with
   | fvar y => grind [LcTm.fvar]
   | app t₁ t₂ _ _ ih₁ ih₂ => grind [LcTm.app]
   | lam L T t _ _ ih =>
-    simp only [substTm_lam]
+    simp only [subst_lam]
     apply_cofinite
     · assumption
-    · grind [openTm_substTm_comm_of_neq]
+    · grind [open_subst_comm_of_neq]
   | tApp t T _ _ ih => grind [LcTm.tApp]
   | tLam L t _ ih =>
-    simp only [substTm_tLam]
+    simp only [subst_tLam]
     apply_cofinite
     intro Y hY
-    rw [←openTmTy_substTm_comm hu]
+    rw [←openTy_subst_comm hu]
     apply ih
     grind
 
 @[aesop safe apply (rule_sets := [LcRules])]
-theorem substTmTy_lcTm {t : Tm} {X : Name} {U : Ty} (ht : LcTm t)
+theorem Tm.substTy_lc {t : Tm} {X : Name} {U : Ty} (ht : LcTm t)
     (hU : LcTy U) : LcTm (t[X ↦ U]) := by
   induction ht generalizing X with ln_norm
 
 @[grind ., aesop unsafe 50% apply (rule_sets := [LcRules])]
-theorem openTm_lcTm {t u : Tm} {T : Ty} (ht : LcTm (ƛ T => t)) (hu : LcTm u) :
+theorem Tm.open_lc {t u : Tm} {T : Ty} (ht : LcTm (ƛ T => t)) (hu : LcTm u) :
     LcTm (t⟪u⟫) := by
   cases ht with
   | lam L T t _ h =>
     pick_fresh x
-    rw [←substTm_openTm_var (x:= x) (by grind)]
+    rw [←subst_open_var (x:= x) (by grind)]
     ln_norm
 
 @[grind ., aesop unsafe 50% apply (rule_sets := [LcRules])]
-theorem openTmTy_lcTm {t : Tm} {U : Ty} (ht : LcTm (Λ' t)) (hU : LcTy U) :
+theorem Tm.openTy_lc {t : Tm} {U : Ty} (ht : LcTm (Λ' t)) (hU : LcTy U) :
     LcTm (t⟪U⟫) := by
   cases ht with
   | tLam L t h =>
     pick_fresh X
-    rw [←substTmTy_openTmTy_var (X := X) (by grind)]
-    grind [substTmTy_lcTm]
+    rw [←substTy_openTy_var (X := X) (by grind)]
+    grind [substTy_lc]
 
-theorem psubst_openTmTy_comm' {t : Tm} {U : Ty} {k} {X : Name} {γ : TmSubst} {δ : TySubst}
+theorem Tm.psubst_openTy_comm_update {t : Tm} {U : Ty} {k} {X : Name} {γ : TmSubst} {δ : TySubst}
     (hX : X ∉ t.fvTy)
     (hγ : ∀ x, LcTm (γ x))
     (hδ : ∀ Y, LcTy (δ Y)) :
     (t.psubst γ δ)⟪k, U⟫ = (t⟪k, $TX⟫).psubst γ (Function.update δ X U) := by
-  induction t generalizing X k with grind [Tm.psubst, openTmTy_lcTm_id, psubst_openTy_comm']
+  induction t generalizing X k with grind [Tm.psubst, Tm.openTy_lc_id, Ty.psubst_open_comm_update]
 
-theorem psubst_openTmTy_comm {t : Tm} {k} {X : Name} {γ : TmSubst} {δ : TySubst}
+theorem Tm.psubst_openTy_comm {t : Tm} {k} {X : Name} {γ : TmSubst} {δ : TySubst}
     (hX : X ∉ t.fvTy)
     (hγ : ∀ x, LcTm (γ x))
     (hδ : ∀ Y, LcTy (δ Y)) :
     (t.psubst γ δ)⟪k, $TX⟫ = (t⟪k, $TX⟫).psubst γ (Function.update δ X ($TX)) := by
-  apply psubst_openTmTy_comm' hX hγ hδ
+  apply psubst_openTy_comm_update hX hγ hδ
 
 @[aesop safe apply (rule_sets := [LcRules])]
 lemma psubst_lcTm {t : Tm} (ht : LcTm t)
@@ -114,10 +115,10 @@ lemma psubst_lcTm {t : Tm} (ht : LcTm t)
   | lam L T t _ _ ih =>
     apply_cofinite
     · apply psubst_lcTy <;> assumption
-    · grind [psubst_openTm_comm, LcTm.fvar]
+    · grind [Tm.psubst_open_comm, LcTm.fvar]
   | tApp t T _ _ _ => grind [Tm.psubst, psubst_lcTy, LcTm.tApp]
   | tLam L t _ ih =>
     apply_cofinite
-    grind [psubst_openTmTy_comm, LcTy.fvar]
+    grind [Tm.psubst_openTy_comm, LcTy.fvar]
 
 end SystemF
